bedrock2/src/bedrock2/Array.v
@@ -133,6 +133,63 @@ Section Array.
 
 End Array.
 
+Require Import coqutil.Map.OfListWord.
+Require Import Ring_tac.
+Section WithWord.
+  Local Coercion Z.of_nat : nat >-> Z.
+  Local Infix "$+" := map.putmany (at level 70).
+  Local Notation "xs $@ a" := (map.of_list_word_at a xs) (at level 10, format "xs $@ a").
+  Local Infix "*" := sep : type_scope.
+  Local Open Scope sep_scope.
+  Context {width : Z} {word : Word.Interface.word width} {word_ok : word.ok word}.
+  Context [value] [map : map.map word value] {ok : map.ok map}.
+  Add Ring __wring: (@word.ring_theory width word word_ok).
+  Lemma sep_eq_of_list_word_at_app (a : word) (xs ys : list value)
+    lxs (Hlxs : Z.of_nat (length xs) = lxs) (Htotal : length xs + length ys <= 2^width)
+    : Lift1Prop.iff1 (eq ((xs ++ ys)$@a))
+      (sep (eq (xs$@a)) (eq (ys$@(word.add a (word.of_Z lxs))))).
+  Proof.
+    etransitivity.
+    2: eapply sep_comm.
+    etransitivity.
+    2: eapply sep_eq_putmany, map.adjacent_arrays_disjoint_n; trivial.
+    erewrite map.of_list_word_at_app_n by eauto; reflexivity.
+  Qed.
+
+  Lemma list_word_at_app_of_adjacent_eq (a b : word) (xs ys : list value)
+    (Hl: word.unsigned (word.sub b a) = Z.of_nat (length xs))
+    (Htotal : length xs + length ys <= 2^width)
+    : Lift1Prop.iff1 (eq(xs$@a)*eq(ys$@b)) (eq((xs++ys)$@a)).
+  Proof.
+    etransitivity.
+    2:symmetry; eapply sep_eq_of_list_word_at_app; trivial.
+    do 3 Morphisms.f_equiv. rewrite <-Hl, word.of_Z_unsigned. ring.
+  Qed.
+
+  Lemma array1_iff_eq_of_list_word_at (a : word) (bs : list value)
+    (H : length bs <= 2 ^ width) :
+    iff1 (array ptsto (word.of_Z 1) a bs) (eq(bs$@a)).
+  Proof.
+    symmetry.
+    revert H; revert a; induction bs; cbn [array]; intros.
+    { rewrite map.of_list_word_nil; cbv [emp iff1]; intuition auto. }
+    { etransitivity.
+      2: eapply Proper_sep_iff1.
+      3: eapply IHbs.
+      2: reflexivity.
+      2: cbn [length] in H; blia.
+      change (a::bs) with (cons a nil++bs).
+      rewrite map.of_list_word_at_app.
+      etransitivity.
+      1: eapply sep_eq_putmany, map.adjacent_arrays_disjoint; cbn [length] in *; blia.
+      etransitivity.
+      2:eapply sep_comm.
+      Morphisms.f_equiv.
+      rewrite map.of_list_word_singleton; try exact _.
+      cbv [ptsto iff1]; intuition auto. }
+  Qed.
+End WithWord.
+
 Require Import Ring.
 
 Section DifferentElemPredicates.
@@ -260,52 +317,49 @@ Section ByteArray.
         symmetry. apply map.putmany_empty_r.
   Qed.
 
-  Lemma array_1_to_anybytes: forall bs m (addr: word),
-      array  addr bs m ->
-      Memory.anybytes addr (Z.of_nat (List.length bs)) m.
+  Lemma sep_ptsto_same [key value] {map : map.map key value} {map_ok : map.ok map}
+    a b c (m : map) : (ptsto a b * ptsto a c)%sep m -> False.
   Proof.
-    unfold Memory.anybytes.
-    intros. eauto using array_1_to_of_disjoint_list_zip.
+    cbv [ptsto]; intros (?&?&[]&?&?); subst.
+    eapply H0; erewrite ?map.get_put_same; eauto.
   Qed.
 
-  Lemma of_disjoint_list_zip_to_array_1: forall n (addr: word) bs m,
-      map.of_disjoint_list_zip (Memory.ftprint addr (Z.of_nat n)) bs = Some m ->
-      array  addr bs m.
+  Lemma sep_ptsto_same_framed [key value] {map : map.map key value} {map_ok : map.ok map}
+    a b c R (m : map) : (ptsto a b * ptsto a c * R)%sep m -> False.
+  Proof. intros (?&?&?&?&?). eapply sep_ptsto_same; eauto. Qed.
+
+  Lemma bytearray_fits_in_address_space bs m addr (H : array addr bs m) :
+    Z.of_nat (length bs) <= 2 ^ width.
   Proof.
-    induction n; intros.
-    - change (Z.of_nat 0) with 0 in *. unfold Memory.ftprint, map.of_disjoint_list_zip in *. simpl in *.
-      destruct bs eqn:?; simpl; subst; unfold emp; intuition congruence.
-    - unfold Memory.ftprint, map.of_disjoint_list_zip in H.
-      rewrite Nat2Z.id in H.
-      simpl in H.
-      do 3 match type of H with match ?x with _ => _ end = _ => destruct x eqn:?; try discriminate end.
-      inversion H; subst; clear H.
-      eapply sep_on_undef_put. 1: assumption. apply IHn. unfold map.of_disjoint_list_zip, Memory.ftprint.
-      rewrite Nat2Z.id.
-      eassumption.
+    pose proof word.width_pos.
+    case (Z.leb_spec (Z.of_nat (length bs)) (2^width)) as []; trivial; exfalso.
+    eapply array_index_nat_inbounds with (n:=Z.to_nat (2^width))(default:=Byte.x00) in H.
+    2:Lia.lia.
+    rewrite word.unsigned_of_Z_1, Z.mul_1_l, Z2Nat.id in H by Lia.lia.
+    erewrite word.of_Z_inj_mod with (x:=2^width)(y:=0), word.add_0_r in H by
+      (rewrite Zdiv.Z_mod_same_full, Zdiv.Zmod_0_l; trivial).
+    case firstn eqn:? in H.
+    { eapply (f_equal (@length _)) in Heql.
+      rewrite firstn_length in *; cbn [length] in *; Lia.lia. }
+    cbn [array] in H.
+    eapply sep_ptsto_same_framed; try exact _; ecancel_assumption.
+  Qed.
+
+  Lemma array_1_to_anybytes: forall bs m (addr: word),
+      array addr bs m ->
+      Memory.anybytes addr (Z.of_nat (List.length bs)) m.
+  Proof.
+    cbv [Memory.anybytes]; intros.
+    split; eauto using Nat2Z.is_nonneg, bytearray_fits_in_address_space; [].
+    eapply array1_iff_eq_of_list_word_at in H; eauto.
+    eauto using bytearray_fits_in_address_space.
   Qed.
 
   Lemma anybytes_to_array_1: forall m (addr: word) n,
       Memory.anybytes addr n m ->
       exists bs, array  addr bs m /\ List.length bs = Z.to_nat n.
   Proof.
-    unfold Memory.anybytes.
-    intros.
-    destruct H as (?&?).
-    assert (n < 0 \/ 0 <= n) as C by blia. destruct C as [C | C]. {
-      destruct n; try blia.
-      unfold Memory.ftprint in H.
-      rewrite Z2Nat.inj_neg in H.
-      simpl in *.
-      unfold map.of_disjoint_list_zip in H. simpl in H. destruct x; try discriminate.
-      exists nil. simpl. unfold emp. intuition congruence.
-    }
-    eexists.
-    epose proof of_disjoint_list_zip_to_array_1 (Z.to_nat n) addr _ m as P.
-    rewrite Z2Nat.id in P by assumption. split; eauto.
-    unfold Memory.ftprint in H.
-    apply map.of_disjoint_list_zip_length in H.
-    rewrite List.length_unfoldn in H.
-    blia.
+    cbv [Memory.anybytes]; intros ? ? ? ([]&?&?&?); subst; eexists; split;
+      try eapply array1_iff_eq_of_list_word_at; eauto using Nat2Z.id.
   Qed.
 End ByteArray.
