bedrock2/src/bedrock2/anybytes.v
@@ -1,0 +1,76 @@
+Require Import Coq.ZArith.ZArith. Local Open Scope Z_scope.
+Require Import Coq.micromega.Lia.
+Require Import coqutil.Word.Interface coqutil.Word.Properties coqutil.Word.Bitwidth.
+Require Import coqutil.Map.Interface.
+Require Import coqutil.Map.Separation.
+Require Import coqutil.Map.OfListWord.
+Require Import bedrock2.Array.
+Require Import bedrock2.Scalars.
+
+Import Init.Byte.
+
+Section WithMem.
+  Context {width} {BW: Bitwidth width} {word: word width} {mem: map.map word Byte.byte}
+          {word_ok: word.ok word} {mem_ok: map.ok mem}.
+
+  Definition anybytes (a : word) (n : Z) (m : mem): Prop :=
+    n <= 2^width /\ 
+    exists bytes, Z.of_nat (length bytes) = n /\ m = map.of_list_word_at a bytes.
+
+  Lemma anybytes_unique_domain: forall a n m1 m2,
+      anybytes a n m1 ->
+      anybytes a n m2 ->
+      map.same_domain m1 m2.
+  Proof.
+    unfold anybytes. intros.
+    destruct H as [vs1 [? []] ]. destruct H0 as [vs2 [? []] ]. subst.
+    cbv [map.same_domain map.sub_domain]; setoid_rewrite map.get_of_list_word_at.
+    split; intros ? ? ?%List.nth_error_Some_bound_index;
+      eexists; eapply List.nth_error_nth'; Lia.lia.
+    Unshelve. all : exact Byte.x00.
+  Qed.
+
+  Local Notation array := (array (mem:=mem) ptsto (word.of_Z 1)).
+  Lemma array_1_to_anybytes: forall bs m (addr: word),
+      array addr bs m ->
+      anybytes addr (Z.of_nat (List.length bs)) m.
+  Proof.
+    cbv [anybytes]; intros.
+    split; eauto using Nat2Z.is_nonneg, bytearray_fits_in_address_space; [].
+    eapply array1_iff_eq_of_list_word_at in H; eauto.
+    eauto using bytearray_fits_in_address_space.
+  Qed.
+
+  Lemma anybytes_to_array_1: forall m (addr: word) n,
+      anybytes addr n m ->
+      exists bs, array  addr bs m /\ List.length bs = Z.to_nat n.
+  Proof.
+    cbv [anybytes]; intros ? ? ? (?&?&?&?); subst; eexists; split;
+      try eapply array1_iff_eq_of_list_word_at; eauto using Nat2Z.id.
+  Qed.
+
+  Lemma scalar_to_anybytes px x:
+    Lift1Prop.impl1 (T := mem)
+      (scalar px x)
+      (anybytes px (Memory.bytes_per_word width)).
+  Proof.
+    intros m H; evar (bs: list byte);
+      assert (array px bs m) by
+        (subst bs; simple apply H).
+    subst bs. erewrite <- bytes_per_width_bytes_per_word, <- split_bytes_per_len.
+    rewrite HList.tuple.to_list_of_list in H0.
+    eapply array_1_to_anybytes; eauto.
+  Qed.
+
+  Lemma anybytes_to_scalar px:
+    Lift1Prop.impl1 (T := mem)
+      (anybytes px (Memory.bytes_per_word width))
+      (Lift1Prop.ex1 (scalar px)).
+  Proof.
+    intros m (bs & Harray & Hlen)%anybytes_to_array_1.
+    apply scalar_of_bytes in Harray.
+    - eexists; eassumption.
+    - rewrite Hlen. clear H. destruct width_cases; subst; reflexivity || lia.
+  Qed.
+
+End WithMem.
